settling on inst_assocs

WebAssembly/Wasm_Instantiation_Monad_Properties.thy
@@ -245,10 +245,10 @@ lemma list_assn_split:"list_assn P xs1 ys1 * list_assn P xs2 ys2
 
 
 lemma interp_alloc_module_m_triple:
-  "< s_m_assn (is', i_ms') s s_m * inst_pile_assn (is, i_ms)>
+  "< s_m_assn (is', i_ms') s s_m * inst_assocs_assn (is, i_ms)>
   interp_alloc_module_m s_m m imps gvs
   <\<lambda>(s_m', i_m, exps_m). let (s', i, exps) = interp_alloc_module s m imps gvs in 
-  \<up>(exps=exps_m) * inst_pile_assn (i#is, i_m#i_ms) * s_m_assn (i#is', i_m#i_ms') s' s_m' >\<^sub>t"
+  \<up>(exps=exps_m) * inst_assocs_assn (i#is, i_m#i_ms) * s_m_assn (i#is', i_m#i_ms') s' s_m' >\<^sub>t"
 proof - 
   
 
@@ -258,7 +258,7 @@ proof -
 
   show ?thesis
   unfolding s_m_assn_def funcs_m_assn_def tabs_m_assn_def 
-    mems_m_assn_def globs_m_assn_def inst_m_assn_def inst_pile_assn_def
+    mems_m_assn_def globs_m_assn_def inst_m_assn_def inst_assocs_assn_def
     (* unfolding and simplifying interp_alloc_module immediately
     to reduce the load on sep_auto later *)
     interp_alloc_module_def alloc_funcs_equiv_full alloc_funcs_simple_conv 
@@ -466,22 +466,22 @@ lemma interp_get_v_m_triple:
   <\<lambda>r.\<up>(r = interp_get_v s inst b_es) 
   * s_m_assn i_s s s_m * inst_m_assn inst inst_m >\<^sub>t"
 proof -
-  note 4 = const_exprs_run_v_m_triple
+  note 1 = const_exprs_run_v_m_triple
     [simplified locs_m_assn_def,
       OF assms]
-  obtain v where 7:"run_v 2 0 (s, \<lparr>f_locs = [], f_inst = inst\<rparr>, b_es) = (s, v)" 
+  obtain v where 2:"run_v 2 0 (s, \<lparr>f_locs = [], f_inst = inst\<rparr>, b_es) = (s, v)" 
     using const_exprs_run_v'[OF assms(1) assms(2)] by auto
   show ?thesis          
     unfolding interp_get_v_m_def interp_get_v_def
     supply [simp del] = run_v_m.simps run_v.simps
-    apply(sep_auto heap:4)
-    apply(sep_auto split:res.splits prod.splits simp:inst_pile_assn_def  7)
+    apply(sep_auto heap:1)
+    apply(sep_auto split:res.splits prod.splits simp:2)
     done 
 qed
 
-lemma inst_pile_assn_cons:
-  "inst_pile_assn (i#is, i_m#i_ms) = inst_pile_assn (is, i_ms) * inst_m_assn i i_m"
-  unfolding inst_pile_assn_def 
+lemma inst_assocs_assn_cons:
+  "inst_assocs_assn (i#is, i_m#i_ms) = inst_assocs_assn (is, i_ms) * inst_m_assn i i_m"
+  unfolding inst_assocs_assn_def 
   by (simp add: assn_times_comm)
 
 lemma interp_get_v_m_triple':
@@ -510,13 +510,13 @@ abbreviation data_in_bounds' where
 
 lemma element_in_bounds_m_triple: 
   assumes "inst_at i_s (i, i_m) j"
-  shows "< s_m_assn i_s' s s_m * inst_pile_assn i_s> 
+  shows "< s_m_assn i_s' s s_m * inst_assocs_assn i_s> 
   element_in_bounds_m s_m i_m e_offs m_elems 
   <\<lambda>r. \<up>(r = list_all2 (element_in_bounds' s i) (map nat_of_int e_offs) m_elems) * 
-  s_m_assn i_s' s s_m * inst_pile_assn i_s>"
+  s_m_assn i_s' s s_m * inst_assocs_assn i_s>"
   using assms 
   unfolding element_in_bounds_m_def s_m_assn_def tabs_m_assn_def 
-    inst_at_def inst_pile_assn_def inst_m_assn_def list_assn_conv_idx 
+    inst_at_def inst_assocs_assn_def inst_m_assn_def list_assn_conv_idx 
   apply(sep_auto split:prod.splits)
   apply(vcg decon:list_all2_m_decon[where Q'="\<lambda>r. _ * \<up>(r = _)"])
      apply(extract_reinsert_list_idx j)
@@ -536,13 +536,13 @@ lemma element_in_bounds_m_triple:
 
 lemma data_in_bounds_m_triple: 
   assumes "inst_at i_s (i, i_m) j"
-  shows "< s_m_assn i_s' s s_m * inst_pile_assn i_s> 
+  shows "< s_m_assn i_s' s s_m * inst_assocs_assn i_s> 
   data_in_bounds_m s_m i_m d_offs m_datas 
   <\<lambda>r. \<up>(r = list_all2 (data_in_bounds' s i) (map nat_of_int d_offs) m_datas) * 
-  s_m_assn i_s' s s_m * inst_pile_assn i_s>"
+  s_m_assn i_s' s s_m * inst_assocs_assn i_s>"
   using assms 
   unfolding data_in_bounds_m_def s_m_assn_def  mems_m_assn_def
-    inst_at_def inst_pile_assn_def inst_m_assn_def list_assn_conv_idx 
+    inst_at_def inst_assocs_assn_def inst_m_assn_def list_assn_conv_idx 
   apply(sep_auto split:prod.splits)
   apply(vcg decon:list_all2_m_decon[where Q'="\<lambda>r. _ * \<up>(r = _)"])
      apply(extract_reinsert_list_idx j)
@@ -564,11 +564,11 @@ abbreviation get_start where "get_start inst st \<equiv>
 
 lemma get_start_m_triple: 
   assumes "inst_at i_s (i, i_m) j"
-  shows "< inst_pile_assn i_s> 
+  shows "< inst_assocs_assn i_s> 
   get_start_m i_m st 
-  <\<lambda>r. \<up>(r = get_start i st) * inst_pile_assn i_s>"
+  <\<lambda>r. \<up>(r = get_start i st) * inst_assocs_assn i_s>"
   using assms 
-  unfolding get_start_m_def inst_at_def inst_pile_assn_def inst_m_assn_def list_assn_conv_idx 
+  unfolding get_start_m_def inst_at_def inst_assocs_assn_def inst_m_assn_def list_assn_conv_idx 
   apply(sep_auto split:prod.splits)
    apply(extract_reinsert_list_idx j)
   apply(sep_auto)
@@ -582,11 +582,11 @@ abbreviation get_init_tabs where "get_init_tabs inst e_inds es \<equiv>
 
 lemma get_init_tab_m_triple: 
   assumes "inst_at i_s (i, i_m) j"
-  shows "< inst_pile_assn i_s> 
+  shows "< inst_assocs_assn i_s> 
   get_init_tab_m i_m e_ind e 
-  <\<lambda>r. \<up>(r = get_init_tab i e_ind e) * inst_pile_assn i_s>"
+  <\<lambda>r. \<up>(r = get_init_tab i e_ind e) * inst_assocs_assn i_s>"
   using assms 
-  unfolding get_init_tab_m_def inst_at_def inst_pile_assn_def inst_m_assn_def list_assn_conv_idx
+  unfolding get_init_tab_m_def inst_at_def inst_assocs_assn_def inst_m_assn_def list_assn_conv_idx
   apply(sep_auto split:prod.splits)
    apply(vcg decon:fold_map_decon'[where Q="\<lambda>x r. \<up>((inst.funcs i)!x = r)"])
     apply(extract_reinsert_list_idx j)
@@ -597,9 +597,9 @@ lemma get_init_tab_m_triple:
 
 lemma get_init_tabs_m_triple: 
   assumes "inst_at i_s (i, i_m) j"
-  shows "< inst_pile_assn i_s> 
+  shows "< inst_assocs_assn i_s> 
   get_init_tabs_m i_m e_inds es 
-  <\<lambda>r. \<up>(r = get_init_tabs i e_inds es) * inst_pile_assn i_s>"
+  <\<lambda>r. \<up>(r = get_init_tabs i e_inds es) * inst_assocs_assn i_s>"
   using assms 
   unfolding get_init_tabs_m_def 
   apply(sep_auto split:prod.splits)
@@ -621,7 +621,7 @@ lemma list_assn_true:"list_assn (\<lambda>x y. true) xs ys =
 lemma list_assn_true':"list_assn (\<lambda>x y. true) xs ys \<Longrightarrow>\<^sub>A true"
   by simp 
                              
-fun res_inst_m_agree :: "inst_pile \<Rightarrow> res_inst \<Rightarrow> res_inst_m \<Rightarrow> bool " where
+fun res_inst_m_agree :: "inst_assocs \<Rightarrow> res_inst \<Rightarrow> res_inst_m \<Rightarrow> bool " where
   "res_inst_m_agree i_s (RI_crash e) (RI_crash_m e_m) = (e = e_m)"
 | "res_inst_m_agree i_s (RI_trap t) (RI_trap_m t_m) = (t = t_m)"
 | "res_inst_m_agree i_s (RI_res i v_exps es) (RI_res_m i_m v_exps_m es_m) = 
@@ -629,10 +629,10 @@ fun res_inst_m_agree :: "inst_pile \<Rightarrow> res_inst \<Rightarrow> res_inst
 | "res_inst_m_agree i_s _ _ = False"
 
 lemma interp_instantiate_m_triple: 
-  "< s_m_assn i_s  s s_m * inst_pile_assn i_s  > 
+  "< s_m_assn i_s  s s_m * inst_assocs_assn i_s  > 
   interp_instantiate_m s_m m v_imps 
   <\<lambda>(s_m', res_m). let (s', res) = interp_instantiate s m v_imps in 
-  \<exists>\<^sub>Ai_s'. \<up>(res_inst_m_agree i_s' res res_m) * s_m_assn i_s' s' s_m' * inst_pile_assn i_s'  >\<^sub>t"
+  \<exists>\<^sub>Ai_s'. \<up>(res_inst_m_agree i_s' res res_m) * s_m_assn i_s' s' s_m' * inst_assocs_assn i_s'  >\<^sub>t"
 proof - 
   obtain iss i_ms where i_s:"i_s = (iss, i_ms)" using surjective_pairing by blast
 
@@ -675,7 +675,7 @@ proof -
       apply(vcg decon:fold_map_decon
         [where R="\<lambda>x. module_elem_typing _ x" and 
           Q="\<lambda>e r.\<up>(interp_get_i32 _ _ (e_off e) = r) * true"])
-       apply(sep_auto simp:inst_pile_assn_def interp_get_i32_m_def interp_get_i32_def
+       apply(sep_auto simp:inst_assocs_assn_def interp_get_i32_m_def interp_get_i32_def
           module_elem_typing.simps inst_at_def 
           heap: interp_get_v_m_triple)
       apply(solve_entails)
@@ -684,7 +684,7 @@ proof -
       apply(vcg decon:fold_map_decon
         [where R="\<lambda>x. module_data_typing _ x" and 
           Q="\<lambda>d r.\<up>(interp_get_i32 _ _ (d_off d) = r) * true"])
-       apply(sep_auto simp:inst_pile_assn_def interp_get_i32_m_def interp_get_i32_def
+       apply(sep_auto simp:inst_assocs_assn_def interp_get_i32_m_def interp_get_i32_def
           module_data_typing.simps inst_at_def 
           heap: interp_get_v_m_triple)
       apply(solve_entails)
@@ -701,10 +701,10 @@ proof -
 qed
 
 lemma interp_instantiate_init_m_triple:
-  "< s_m_assn i_s s s_m * inst_pile_assn i_s> 
+  "< s_m_assn i_s s s_m * inst_assocs_assn i_s> 
   interp_instantiate_init_m s_m m v_imps
   <\<lambda>(s_m', res_m). let (s', res) = interp_instantiate_init s m v_imps in 
-  \<exists>\<^sub>Ai_s'. \<up>(res_inst_m_agree i_s' res res_m) * s_m_assn i_s' s' s_m' * inst_pile_assn i_s' >\<^sub>t" 
+  \<exists>\<^sub>Ai_s'. \<up>(res_inst_m_agree i_s' res res_m) * s_m_assn i_s' s' s_m' * inst_assocs_assn i_s' >\<^sub>t" 
   unfolding interp_instantiate_init_m_def interp_instantiate_init_def 
   supply [simp del] = interp_instantiate_m.simps interp_instantiate.simps
     run_instantiate_m.simps run_instantiate.simps
